complete ex2_down

theories/opt/ex2_down.v
@@ -1,13 +1,13 @@
-From stbor.sim Require Import local invariant refl_step.
+From stbor.sim Require Import local invariant refl.
 From stbor.sim Require Import tactics simple program.
-From stbor.sim Require Import refl_step right_step left_step viewshift.
+From stbor.sim Require Import refl_step right_step left_step derived_step viewshift.
 
 Set Default Proof Using "Type".
 
 (** Moving a read of a shared reference down across code that *may* use that ref. *)
 
 (* Assuming x : & i32 *)
-Definition ex2_down : function :=
+Definition ex2_down_unopt : function :=
   fun: ["i"],
     let: "x" := new_place (& int) "i" in
     retag_place "x" (RefPtr Immutable) int FnEntry ;;
@@ -28,24 +28,139 @@ Definition ex2_down_opt : function :=
   .
 
 
-Lemma ex2_down_sim_fun : ⊨ᶠ ex2_down ≥ ex2_down_opt.
+Lemma ex2_down_sim_fun : ⊨ᶠ ex2_down_unopt ≥ ex2_down_opt.
 Proof.
-  apply (sim_fun_simple1 10)=>// fs ft rarg es et arg c LOOK AREL ??.
-  simplify_eq/=.
+  (* We can't use sim_simple because we need to track our stack frame id *)
+  intros fs ft LOOK rarg es et vls vlt σs σt FREL SUBSTs SUBSTt.
+  (* Substitution *)
+  move:(subst_l_is_Some_length _ _ _ _ SUBSTs) (subst_l_is_Some_length _ _ _ _ SUBSTt).
+  rewrite /= => Hls Hlt.
+  destruct vls as [|vs []]; [done| |done].
+  destruct vlt as [|arg []]; [done| |done]. clear Hls Hlt.
+  inversion FREL as [|???? VREL _].
+  clear FREL. specialize (vrel_eq _ _ _ VREL)=>?.
+  simplify_eq. simpl in SUBSTs, SUBSTt. simplify_eq/=.
+  (* Init call *)
+  exists 10%nat. apply sim_body_init_call=>/= Eqcs.
   (* Alloc local *)
-  sim_apply sim_simple_alloc_local=> l t /=.
-  sim_apply sim_simple_let=>/=.
+  sim_apply sim_body_alloc_local => /=.
+  sim_apply sim_body_let=>/=.
   (* Write local *)
-  sim_apply sim_simple_write_local; [solve_sim..|].
-  intros sarg ->.
-  sim_apply sim_simple_let=>/=.
-  apply: sim_simple_result.
+  sim_apply sim_body_write_local_1; [solve_sim..|].
+  intros sarg ? σs1 σt1. subst arg.
+  sim_apply sim_body_let=>/=.
+  apply: sim_body_result => _.
   (* Retag a local place *)
-  sim_apply sim_simple_let=>/=.
-  apply Forall2_cons_inv in AREL as [AREL _].
-  sim_apply sim_simple_let=>/=.
+  sim_apply sim_body_let=>/=.
+  apply Forall2_cons_inv in VREL as [AREL _].
+  sim_apply sim_body_let=>/=.
     (* Copy local place *)
-    sim_apply sim_simple_copy_local; [solve_sim..|].
-    apply sim_simple_valid_post.
-    apply: sim_simple_result. simpl. intros VALID.
-Abort.
+    sim_apply sim_body_copy_local; [solve_sim..|].
+    sim_apply sim_body_result => /= VALID.
+    (* Retag *)
+    sim_apply sim_body_retag_ref_fn_entry; [simpl; lia|eauto| |done|..].
+    { rewrite -cmra_assoc (cmra_comm (res_cs _ _)) cmra_assoc. eauto. }
+    { eapply arel_mono; [done|..|exact AREL]. solve_res. } clear VALID.
+    move=> l' told tnew hplt α' nxtp' r0 ? _ IS_i InD σs2 σt2 s_new tk ARELn /=.
+    subst sarg.
+    have IS_O := (IS_i O ltac:(simpl; lia)). rewrite shift_loc_0_nat in IS_O.
+    destruct IS_O as [(ss & st & Eql' & Eqss & Eqst & ARELs) TOP].
+    rewrite insert_empty.
+    (* Write local *)
+    sim_apply sim_body_write_local_1; [solve_sim..|].
+    intros s ?. simplify_eq. simpl.
+  sim_apply sim_body_let=>/=.
+  (* Copy local left *)
+  sim_apply_l sim_body_copy_local_l; [solve_sim..|].
+  apply: sim_body_result=>_ /=.
+  (* Copy unique left *)
+  sim_apply_l sim_body_deref_l =>/=.
+  sim_apply_l sim_body_copy_public_l; [solve_sim..|].
+  move => r' ARELs'.
+  apply: sim_body_result=>_/=.
+  apply: sim_body_let_l=>/=.
+  (* Copy local place *)
+  sim_apply sim_body_copy_local; [solve_sim..|].
+  apply: sim_body_result=>_/=.
+  (* Call *)
+  set r1 := rarg ⋅ res_cs σt.(snc) {[tnew := dom (gset loc) hplt]} ⋅
+            res_tag tnew tk hplt ⋅ r0 ⋅
+            res_loc (fresh_block σt.(shp), 0)
+                    [(ScPtr l' (Tagged tnew), ScPtr l' (Tagged tnew))] σt.(snp) ⋅
+            r'.
+  rewrite (_: r1 ≡ r1 ⋅ res_tag tnew tk hplt); last first.
+  { rewrite /r1 {1}res_tag_public_dup cmra_assoc. solve_res. }
+  sim_bind (Call _ _) (Call _ _). (* TODO: sim_apply fails to instantiate evars *)
+  apply (sim_body_step_over_call _ _ _ (res_tag tnew tkPub hplt) _ (ValR _)
+              [ValR [ScPtr l' (Tagged tnew)]] [ValR [ScPtr l' (Tagged tnew)]]);
+    [|done|].
+  { constructor; [|by constructor].
+    constructor; [done|by constructor]. } clear ARELn.
+  move => rf' ? _ _ frs' frt' σs3 σt3 _ /= Eqs1 Eqs2 ? _ _. simplify_eq.
+  exists 5%nat.
+  apply: sim_body_result=>_ /=.
+  sim_apply sim_body_let=>/=. clear frs' frt'.
+  (* Copy local right *)
+  sim_apply_r sim_body_copy_local_r; [|rewrite /r1|..]; [solve_sim..|].
+  apply: sim_body_result=>_ /=.
+  (* Copy protected right *)
+  sim_apply_r sim_body_deref_r =>/=.
+  sim_apply_r sim_body_copy_protected_r; [|rewrite /r1|..];
+    [solve_sim..|by rewrite lookup_insert|by eapply elem_of_dom_2|].
+  intros Eqss3 Eqst3.
+  apply: sim_body_result=> Hval /=.
+  apply: sim_body_let_r=>/=.
+  (* Free stuff *)
+  sim_apply sim_body_free_unique_local_1;
+    [done|rewrite /r1 /res_loc /= insert_empty; solve_sim |by left|].
+  move => _ _ α4 _ σs4 σt4.
+  sim_apply sim_body_let=>/=.
+  (* Remove protection *)
+  set r2 := rarg ⋅ r0 ⋅ res_cs σt.(snc) {[tnew := dom (gset loc) hplt]} ⋅
+              res_tag tnew tk hplt ⋅ r' ⋅ rf'.
+  set r3 := rarg ⋅ r0 ⋅ res_cs σt.(snc) ∅ ⋅ res_tag tnew tk hplt ⋅ r' ⋅ rf'.
+  rewrite (_: rarg ⋅ res_cs σt.(snc) {[tnew := dom (gset loc) hplt]} ⋅
+              res_tag tnew tk hplt ⋅ r0 ⋅ r' ⋅ rf' ≡ r2); last first.
+  { rewrite -2!cmra_assoc (cmra_comm r0) cmra_assoc (cmra_comm _ r0)
+            !cmra_assoc (cmra_comm r0) //. }
+  apply (viewshift_state_sim_local_body _ _ _ _ r2 r3).
+  { rewrite /r2 /r3. do 3 apply viewshift_state_frame_r.
+    rewrite -insert_empty. apply vs_state_drop_protector; [done|].
+    move => l1 /InD [i [/= Lti ?]]. subst l1.
+    destruct i; [|clear -Lti; by lia]. rewrite shift_loc_0_nat.
+    move => ss4 /= /lookup_delete_Some [? Eqst4].
+    rewrite Eqst4 in Eqst3. simplify_eq. exists ss.
+    rewrite lookup_delete_ne; [|done]. split; [done|].
+    move : ARELs. apply arel_mono; [|solve_res]. clear -Hval.
+    apply (cmra_valid_included _ _ Hval).
+    do 3 (etrans; [|apply cmra_included_l]).
+    apply cmra_mono_r. solve_res. } clear Hval.
+  (* Finishing up. *)
+  apply: sim_body_result => Hval. split.
+  - exists σt.(snc). split; [done|]. rewrite /end_call_sat.
+    apply (cmap_lookup_op_unique_included (res_cs σt.(snc) ∅).(rcm));
+      [apply Hval|apply prod_included; rewrite /r3; solve_res|..].
+    by rewrite res_cs_lookup.
+  - constructor; [|by constructor].
+    move : ARELs. rewrite /r3. apply arel_mono; [done|solve_res].
+Qed.
+
+(** Top-level theorem: Two programs that only differ in the
+"ex2_down" function are related. *)
+Corollary ex2_down (prog: fn_env) :
+  stuck_decidable →
+  prog_wf prog →
+  let prog_src := <["ex2_down":=ex2_down_unopt]> prog in
+  let prog_tgt := <["ex2_down":=ex2_down_opt]> prog in
+  behave_prog prog_tgt <1= behave_prog prog_src.
+Proof.
+  intros Hdec Hwf. apply sim_prog_sim_classical.
+  { apply Hdec. }
+  { apply has_main_insert, Hwf; done. }
+  apply sim_mod_funs_local.
+  apply sim_mod_funs_insert; first done.
+  - exact: ex2_down_sim_fun.
+  - exact: sim_mod_funs_refl.
+Qed.
+
+Print Assumptions ex2_down.
